kore/src/theories/DemoGen2.v
@@ -1,0 +1,285 @@
+
+
+From MatchingLogic Require Export stdpp_ext.
+From Kore Require Export Semantics.
+Import Signature.StringVariables.
+Import Kore.Syntax.Notations.
+
+From Coq Require Import ZArith.
+
+Open Scope kore_scope.
+Open Scope string_scope.
+Open Scope hlist_scope.
+
+      Module TheorySyntax.
+
+
+Inductive Ksorts :=
+  | SortS1
+| SortS3
+| SortE
+| SortS2
+.
+      Instance Ksorts_eq_dec : EqDecision Ksorts.
+      Proof. solve_decision. Defined.
+      Program Instance Ksorts_countable : finite.Finite Ksorts :=
+      {
+        enum := [SortS1; SortS3; SortE; SortS2]
+      }.
+      Next Obligation.
+        compute_done.
+      Defined.
+      Final Obligation.
+        intros. destruct x; set_solver.
+      Defined.
+
+
+
+Inductive Ksyms :=
+  | syme1
+| syme2
+| syme3
+| symf
+| symg
+| syms2
+| syms3
+.
+      Instance Ksyms_eq_dec : EqDecision Ksyms.
+      Proof. solve_decision. Defined.
+      Program Instance Ksyms_countable : finite.Finite Ksyms :=
+      {
+        enum := [syme1; syme2; syme3; symf; symg; syms2; syms3]
+      }.
+      Next Obligation.
+        compute_done.
+      Defined.
+      Final Obligation.
+        intros. destruct x; set_solver.
+      Defined.
+
+        Inductive KSubsort : CRelationClasses.crelation Ksorts :=
+|  inj_SortS3_SortS1 : KSubsort SortS3 SortS1
+|  inj_SortS2_SortS1 : KSubsort SortS2 SortS1
+|  inj_SortS3_SortS2 : KSubsort SortS3 SortS2
+.
+  Goal forall s1 s2 s3, KSubsort s1 s2 -> KSubsort s2 s3 -> KSubsort s1 s3.
+  Proof.
+    intros ??? H1 H2; inversion H1; inversion H2; try constructor; subst; try discriminate.
+  Defined.
+  Goal forall s1 s2, KSubsort s1 s2 -> KSubsort s2 s1 -> s1 = s2.
+  Proof.
+    intros ?? H H0; inversion H; subst; inversion H0; subst.
+  Defined.
+
+
+Program Instance TheorySignature : Signature := {|
+  sorts := {|
+    sort := Ksorts;
+    subsort := KSubsort;
+  |};
+  variables := StringVariables;
+  symbols := {|
+    symbol := Ksyms;
+    arg_sorts σ :=
+      match σ with
+                | syme1 => []
+  | syme2 => []
+  | syme3 => []
+  | symf => [SortS1]
+  | symg => [SortS1]
+  | syms2 => []
+  | syms3 => []
+      end;
+    ret_sort σ :=
+      match σ with
+                | syme1 => SortE
+  | syme2 => SortE
+  | syme3 => SortE
+  | symf => SortE
+  | symg => SortE
+  | syms2 => SortS2
+  | syms3 => SortS3
+      end;
+  |};
+|}.
+
+Definition Theory_behavioural : @Theory TheorySignature :=
+  PropSet (fun pat =>
+
+(* symf *)
+(exists R, pat = existT R (( ( Top{R} ) and ( ( ( @kore_fevar _ _ _ SortS1 "X0" ) ⊆k{R} ( @kore_fevar _ _ _ SortS1 "Var'Unds'Gen0" ) ) and ( Top{R} ) ) ) --->ₖ ( ( symf ⋅ ⟨@kore_fevar _ _ _ SortS1 "X0"⟩ ) =k{R} ( ( syme1 ⋅ ⟨⟩ ) and ( Top{SortE} ) ) ) )) \/
+
+(* symf *)
+(exists R, pat = existT R (( ( Top{R} ) and ( ( ( @kore_fevar _ _ _ SortS1 "X0" ) ⊆k{R} ( kore_inj _ inj_SortS2_SortS1 (@kore_fevar _ _ _ SortS2 "Var'Unds'Gen0") ) ) and ( Top{R} ) ) ) --->ₖ ( ( symf ⋅ ⟨@kore_fevar _ _ _ SortS1 "X0"⟩ ) =k{R} ( ( syme1 ⋅ ⟨⟩ ) and ( Top{SortE} ) ) ) )) \/
+
+(* symf *)
+(exists R, pat = existT R (( ( Top{R} ) and ( ( ( @kore_fevar _ _ _ SortS1 "X0" ) ⊆k{R} ( kore_inj _ inj_SortS3_SortS1 (@kore_fevar _ _ _ SortS3 "Var'Unds'Gen0") ) ) and ( Top{R} ) ) ) --->ₖ ( ( symf ⋅ ⟨@kore_fevar _ _ _ SortS1 "X0"⟩ ) =k{R} ( ( syme1 ⋅ ⟨⟩ ) and ( Top{SortE} ) ) ) )) \/
+
+(* symg *)
+(exists R, pat = existT R (( ( Top{R} ) and ( ( ( @kore_fevar _ _ _ SortS1 "X0" ) ⊆k{R} ( kore_inj _ inj_SortS3_SortS1 (syms3 ⋅ ⟨⟩) ) ) and ( Top{R} ) ) ) --->ₖ ( ( symg ⋅ ⟨@kore_fevar _ _ _ SortS1 "X0"⟩ ) =k{R} ( ( syme1 ⋅ ⟨⟩ ) and ( Top{SortE} ) ) ) )) \/
+
+(* symg *)
+(exists R, pat = existT R (( ( Top{R} ) and ( ( ( @kore_fevar _ _ _ SortS1 "X0" ) ⊆k{R} ( kore_inj _ inj_SortS3_SortS1 (syms3 ⋅ ⟨⟩) ) ) and ( Top{R} ) ) ) --->ₖ ( ( symg ⋅ ⟨@kore_fevar _ _ _ SortS1 "X0"⟩ ) =k{R} ( ( syme1 ⋅ ⟨⟩ ) and ( Top{SortE} ) ) ) )) \/
+
+(* symg *)
+(exists R, pat = existT R (( ( Top{R} ) and ( ( ( @kore_fevar _ _ _ SortS1 "X0" ) ⊆k{R} ( kore_inj _ inj_SortS3_SortS1 (syms3 ⋅ ⟨⟩) ) ) and ( Top{R} ) ) ) --->ₖ ( ( symg ⋅ ⟨@kore_fevar _ _ _ SortS1 "X0"⟩ ) =k{R} ( ( syme1 ⋅ ⟨⟩ ) and ( Top{SortE} ) ) ) ))
+  ).
+
+Definition Theory_functional : @Theory TheorySignature :=
+  PropSet (fun pat =>
+
+(* syme1 is functional *)
+(exists R, pat = existT R (kore_exists SortE (( kore_bevar (In_nil) ) =k{R} ( syme1 ⋅ ⟨⟩ )) )) \/
+
+(* syme2 is functional *)
+(exists R, pat = existT R (kore_exists SortE (( kore_bevar (In_nil) ) =k{R} ( syme2 ⋅ ⟨⟩ )) )) \/
+
+(* syme3 is functional *)
+(exists R, pat = existT R (kore_exists SortE (( kore_bevar (In_nil) ) =k{R} ( syme3 ⋅ ⟨⟩ )) )) \/
+
+(* syms2 is functional *)
+(exists R, pat = existT R (kore_exists SortS2 (( kore_bevar (In_nil) ) =k{R} ( syms2 ⋅ ⟨⟩ )) )) \/
+
+(* syms3 is functional *)
+(exists R, pat = existT R (kore_exists SortS3 (( kore_bevar (In_nil) ) =k{R} ( syms3 ⋅ ⟨⟩ )) ))
+  ).
+
+      End TheorySyntax.
+      Module TheorySemantics.
+        Import TheorySyntax.
+
+      Inductive SortS1_carrier : Set :=
+ | c_inj_SortS2_SortS1 (b : SortS2_carrier)
+ | c_inj_SortS3_SortS1 (b : SortS3_carrier)
+with SortS3_carrier : Set :=
+ | c_syms3
+with SortE_carrier : Set :=
+ | c_syme1
+ | c_syme2
+ | c_syme3
+with SortS2_carrier : Set :=
+ | c_syms2
+ | c_inj_SortS3_SortS2 (b : SortS3_carrier)
+.
+
+      Definition carrier (s : Ksorts) : Set := match s with
+      SortS1 => SortS1_carrier
+|SortS3 => SortS3_carrier
+|SortE => SortE_carrier
+|SortS2 => SortS2_carrier
+      end.
+
+
+Definition retr_SortS1_SortS3 x := match x with
+  | c_inj_SortS3_SortS1 x => Some x
+  | _ => None
+end.
+
+Definition retr_SortS1_SortS2 x := match x with
+  | c_inj_SortS3_SortS1 x => Some (c_inj_SortS3_SortS2 x)
+  | c_inj_SortS2_SortS1 x => Some x
+end.
+
+Definition retr_SortS2_SortS3 x := match x with
+  | c_inj_SortS3_SortS2 x => Some x
+  | _ => None
+end.
+
+      Definition _0b14131 : SortS1_carrier -> option SortE_carrier
+  := fun x => match x with | c_inj_SortS3_SortS1 c_syms3 => Some c_syme1
+  | _ => None end.
+Definition _b468026 : SortS1_carrier -> option SortE_carrier
+  := fun x => match x with | c_inj_SortS3_SortS1 c_syms3 => Some c_syme1
+  | _ => None end.
+Definition _c0bcf68 : SortS1_carrier -> option SortE_carrier
+  := fun x => match x with | c_inj_SortS3_SortS1 c_syms3 => Some c_syme1
+  | _ => None end.
+Definition _8ab4f38 : SortS1_carrier -> option SortE_carrier
+  := fun x => match x with | _Gen0 => Some c_syme1 end.
+Definition _59f3cb7 : SortS1_carrier -> option SortE_carrier
+  := fun x => match x with | c_inj_SortS3_SortS1 _Gen0 => Some c_syme1
+  | _ => None end.
+Definition _4db77ad : SortS1_carrier -> option SortE_carrier
+  := fun x => match x with | _Pat0 => match (retr_SortS1_SortS2) _Pat0 with
+    | Some _Gen0 => Some c_syme1
+    | _ => None end end.
+Definition symg (x0 : SortS1_carrier) : option SortE_carrier := (_0b14131 x0) <|> (_b468026 x0) <|> (_c0bcf68 x0).
+Definition symf (x0 : SortS1_carrier) : option SortE_carrier := (_4db77ad x0) <|> (_59f3cb7 x0) <|> (_8ab4f38 x0).
+      Program Definition Model : @Model TheorySignature :=
+        mkModel_partial
+          (Ksorts_rect _ SortS1_carrier SortS3_carrier SortE_carrier SortS2_carrier)
+          (Ksyms_rect _ (Some c_syme1) (Some c_syme2) (Some c_syme3) symf symg (Some c_syms2) (Some c_syms3))
+          _ _.
+      Next Obligation.
+        destruct s; repeat constructor.
+      Defined.
+      Final Obligation.
+        intros s1 s2 H x; inversion H; subst.
+      * exact (c_inj_SortS3_SortS1 x).
+* exact (c_inj_SortS2_SortS1 x).
+* exact (c_inj_SortS3_SortS2 x).
+Defined.
+
+Ltac autorewrite_set :=
+  repeat (
+    rewrite intersection_top_l_L +
+    rewrite intersection_top_r_L +
+    rewrite union_empty_l_L +
+    rewrite union_empty_r_L +
+    rewrite propset_difference_neg +
+    rewrite propset_union_simpl +
+    rewrite propset_intersection_simpl +
+    rewrite singleton_subseteq_l +
+    rewrite fmap_propset_singleton
+  ).
+
+Ltac basic_simplify_krule :=
+  eval_helper2;
+  simpl sort_inj;
+  repeat (rewrite_app_ext; repeat rewrite fmap_propset_singleton);
+  autorewrite_set.
+
+Ltac simplify_krule :=
+  basic_simplify_krule;
+  apply propset_top_elem_of_2;
+  intro;
+  apply elem_of_PropSet;
+  repeat rewrite elem_of_PropSet;
+  repeat rewrite singleton_subseteq;
+  repeat rewrite singleton_eq.
+
+Ltac classicize :=
+  apply Classical_Prop.imply_to_or.
+
+Ltac simplify_equality :=
+match goal with
+      | [H : _ _ = _ _ |- _] => simplify_eq H; clear H; intro
+      end.
+
+Ltac abstract_var := 
+  match goal with
+    | [|- context [evar_valuation ?σ ?s]] =>
+      let x := fresh "var" in
+      let Hx := fresh "Hvar" in
+        remember (evar_valuation σ s) as x eqn:Hx (*;
+        clear Hx;
+        revert x *)
+    end.
+
+
+  Goal satT Theory_behavioural Model.
+  Proof.
+    unfold satT, satM. intros.
+    unfold Theory_behavioural in H.
+    unfold_elem_of; destruct_or?; destruct_ex?; subst.
+    all: simplify_krule; try reflexivity;
+         try classicize;
+         intros;
+         repeat destruct_evar_val; subst;
+         repeat simplify_equality; subst;
+         try tauto;
+         try congruence.
+  Defined.
+
+      End TheorySemantics.
+
